src/FlatImp.v
@@ -4,14 +4,10 @@ Require Import compiler.Tactics.
 Require Import compiler.ResMonad.
 Require Import compiler.Op.
 Require Import compiler.StateCalculus.
-Require Import compiler.zcast.
 
 Section FlatImp.
 
   Context {w: nat}. (* bit width *)
-  Context {wlit: nat}. (* max bit width of literals *)
-  Context {wdiff: nat}. (* difference between literal width and word width *)
-  Context {w_eq: wlit + wdiff = w}.
   Context {var: Set}.
   Context {eq_var_dec: DecidableEq var}.
   Context {state: Type}.
@@ -20,7 +16,7 @@ Section FlatImp.
   Context {varset: set vars var}.
 
   Inductive stmt: Set :=
-    | SLit(x: var)(v: word wlit): stmt
+    | SLit(x: var)(v: word w): stmt
     | SOp(x: var)(op: binop)(y z: var): stmt
     | SSet(x y: var): stmt
     | SIf(cond: var)(bThen bElse: stmt): stmt
@@ -39,8 +35,6 @@ Section FlatImp.
     | SSkip => 1
     end.
 
-  Definition signed_lit_to_word(v: word wlit): word w := nat_cast word w_eq (sext v wdiff).
-
   (* If we want a bigstep evaluation relation, we either need to put
      fuel into the SLoop constructor, or give it as argument to eval *)
   Fixpoint eval_stmt(f: nat)(st: state)(s: stmt): Res state :=
@@ -48,7 +42,7 @@ Section FlatImp.
     | 0 => OutOfFuel
     | Coq.Init.Datatypes.S f' => match s with
       | SLit x v =>
-          Success (put st x (signed_lit_to_word v))
+          Success (put st x v)
       | SOp x op y z =>
           v1 <- option2res (get st y);
           v2 <- option2res (get st z);
@@ -74,7 +68,7 @@ Section FlatImp.
 
   Lemma invert_eval_SLit: forall fuel initial x v final,
     eval_stmt fuel initial (SLit x v) = Success final ->
-    final = put initial x (signed_lit_to_word v).
+    final = put initial x v.
   Proof.
     intros. destruct fuel; [discriminate|]. inversion H. auto.
   Qed.
@@ -601,7 +595,7 @@ Example fib(n: word 8) :=
               (SOp _n OMinus _n _one)))))
   )))).
 
-Definition eval_stmt_test := @eval_stmt 8 8 0 eq_refl var _ _.
+Definition eval_stmt_test := @eval_stmt 8 var _ _.
 
 Example finalFibState(n: nat): Res (var -> option (word 8)) := (eval_stmt_test 100 empty (fib $n)).
 Example finalFibVal(n: nat): option (word 8) := match finalFibState n with
